implemented type declarations

Semant.v
@@ -159,19 +159,19 @@ End HELPERS.
 
 Section TYPE_CHECK.
 
-  Definition transOp (lty rty : expty) (f : opType) : @res expty:=
-    if Types.ty_compat (ty lty) (ty rty)
+  Definition transOp (lty rty : Types.ty) (f : opType) : @res expty:=
+    if Types.ty_compat lty rty
       then match f with
-      | Arith => match (ty lty) with
+      | Arith => match lty with
           | Types.INT => OK (mk_expty Types.INT)
           | _ => ERR
           end
-      | Ineq => match (ty lty) with
+      | Ineq => match lty with
           | Types.INT => OK (mk_expty Types.INT)
           | Types.STRING => OK (mk_expty Types.INT)
           | _ => ERR
           end
-      | Eq => match (ty lty) with
+      | Eq => match lty with
           | Types.INT => OK (mk_expty Types.INT)
           | Types.STRING => OK (mk_expty Types.INT)
           | Types.RECORD _ _ => OK (mk_expty Types.INT)
@@ -202,6 +202,21 @@ Section TYPE_CHECK.
                       OK (Types.ARRAY ty u, us')
     end.
 
+  Fixpoint transTydecHeads (te : tenv) (decs : list Absyn.tydec) : @res tenv :=
+    match decs with
+    | nil => OK te
+    | dec :: decs' => let te' := Symbol.enter te (td_name dec) (Types.NAME (td_name dec)) in
+                      transTydecHeads te' decs'
+    end.
+
+  Fixpoint transTydecs (te : tenv) (us : Types.upool) (decs : list Absyn.tydec) : @res (tenv * Types.upool) :=
+    match decs with
+    | nil => OK (te, us)
+    | dec :: decs' => do (dty, us') <- transTy te us (td_ty dec);
+                      let te' := Symbol.enter te (td_name dec) dty in
+                      transTydecs te' us' decs'
+    end.
+
   Fixpoint transExp (ce : composite_env) (us : Types.upool) (exp : Absyn.exp) : @res (expty * Types.upool) :=
     match exp with
     | VarExp v => transVar ce us v
@@ -212,21 +227,27 @@ Section TYPE_CHECK.
                        match entry with
                        | Env.FunEntry formtys retty =>
                            do (argtys, us') <- transExplist ce us args;
-                           check tys_compat (map ty argtys) formtys;
+                           do formtys' <- lift (Types.actual_tys (te ce) formtys);
+                           do argtys' <- lift (Types.actual_tys (te ce) (map ty argtys));
+                           check tys_compat argtys' formtys';
                            OK (mk_expty retty, us')
                        | _ => ERR
                        end
     | OpExp l f r => do (lty, us') <- transExp ce us l;
                      do (rty, us'') <- transExp ce us' r;
-                     do ty <- transOp lty rty (getOpType f);
+                     do lty' <- lift (Types.actual_ty (te ce) (ty lty));
+                     do rty' <- lift (Types.actual_ty (te ce) (ty rty));
+                     do ty <- transOp lty' rty' (getOpType f);
                      OK (ty, us'')
     | RecordExp fvals fnames rty => do recty <- lift (Symbol.look (te ce) rty);
-                                    do recty' <- lift (Types.actual_ty recty);
+                                    do recty' <- lift (Types.actual_ty (te ce) recty);
                                     match recty' with
                                     | Types.RECORD fields _ =>
                                         check syms_eq fnames (map Types.rf_name fields);
                                         do (etys, us') <- transExplist ce us fvals;
-                                        check tys_compat (map ty etys) (map Types.rf_type fields);
+                                        do etys' <- lift (Types.actual_tys (te ce) (map ty etys));
+                                        do fieldtys <- lift (Types.actual_tys (te ce) (map Types.rf_type fields));
+                                        check tys_compat etys' fieldtys;
                                         OK (mk_expty recty', us')
                                     | _ => ERR
                                     end
@@ -234,7 +255,9 @@ Section TYPE_CHECK.
                    OK (last etys (mk_expty Types.UNIT), us')
     | AssignExp l r => do (vty, us') <- transVar ce us l;
                        do (ety, us'') <- transExp ce us' r;
-                       check Types.ty_compat (ty vty) (ty ety);
+                       do vty' <- lift (Types.actual_ty (te ce) (ty vty));
+                       do ety' <- lift (Types.actual_ty (te ce) (ty ety));
+                       check Types.ty_compat vty' ety';
                        match Symbol.look (ro ce) (getVarName l) with
                        | None => OK (mk_expty Types.UNIT, us'')
                        | _ => ERR
@@ -242,27 +265,37 @@ Section TYPE_CHECK.
     | IfExp p t (Some e) => do (pty, us') <- transExp ce us p;
                             do (tty, us'') <- transExp ce us' t;
                             do (ety, us''') <- transExp ce us'' e;
-                            check Types.ty_compat (ty pty) Types.INT;
-                            check Types.ty_compat (ty tty) (ty ety);
+                            do pty' <- lift (Types.actual_ty (te ce) (ty pty));
+                            do tty' <- lift (Types.actual_ty (te ce) (ty tty));
+                            do ety' <- lift (Types.actual_ty (te ce) (ty ety));
+                            check Types.ty_compat pty' Types.INT;
+                            check Types.ty_compat tty' ety';
                             OK (tty, us''')
     | IfExp p t None => do (pty, us') <- transExp ce us p;
                         do (tty, us'') <- transExp ce us' t;
-                        check Types.ty_compat (ty pty) Types.INT;
-                        check Types.ty_compat (ty tty) Types.UNIT;
+                        do pty' <- lift (Types.actual_ty (te ce) (ty pty));
+                        do tty' <- lift (Types.actual_ty (te ce) (ty tty));
+                        check Types.ty_compat pty' Types.INT;
+                        check Types.ty_compat tty' Types.UNIT;
                         OK (mk_expty Types.UNIT, us'')
     | WhileExp g b => do (gty, us') <- transExp ce us g;
                       do (bty, us'') <- transExp (incr_ll ce) us' b;
-                      check Types.ty_compat (ty gty) Types.INT;
-                      check Types.ty_compat (ty bty) Types.UNIT;
+                      do gty' <- lift (Types.actual_ty (te ce) (ty gty));
+                      do bty' <- lift (Types.actual_ty (te ce) (ty bty));
+                      check Types.ty_compat gty' Types.INT;
+                      check Types.ty_compat bty' Types.UNIT;
                       OK (mk_expty Types.UNIT, us'')
     | ForExp v lo hi b => do (loty, us') <- transExp ce us lo;
                           do (hity, us'') <- transExp ce us' hi;
-                          check Types.ty_compat (ty loty) Types.INT;
-                          check Types.ty_compat (ty hity) Types.INT;
+                          do loty' <- lift (Types.actual_ty (te ce) (ty loty));
+                          do hity' <- lift (Types.actual_ty (te ce) (ty hity));
+                          check Types.ty_compat loty' Types.INT;
+                          check Types.ty_compat hity' Types.INT;
                           let ve' := Symbol.enter (ve ce) (vd_name v) (Env.VarEntry Types.INT) in
                           let ro' := Symbol.enter (ro ce) (vd_name v) tt in
                           do (bty, us''') <- transExp (incr_ll (update_ve (update_ro ce ro') ve')) us'' b;
-                          check Types.ty_compat (ty bty) Types.UNIT;
+                          do bty' <- lift (Types.actual_ty (te ce) (ty bty));
+                          check Types.ty_compat bty' Types.UNIT;
                           OK (mk_expty Types.UNIT, us''')
     | BreakExp => check leb 1 (ll ce);
                   OK (mk_expty Types.UNIT, us)
@@ -270,12 +303,16 @@ Section TYPE_CHECK.
                        do (bty, us'') <- transExp ce' us' b;
                        OK (bty, us'')
     | ArrayExp aty sz init => do arrty <- lift (Symbol.look (te ce) aty);
+                              do arrty' <- lift (Types.actual_ty (te ce) arrty);
                               do (szty, us') <- transExp ce us sz;
                               do (initty, us'') <- transExp ce us' init;
-                              check Types.ty_compat (ty szty) Types.INT;
-                              match arrty with
-                              | Types.ARRAY elty _ => check Types.ty_compat (ty initty) elty;
-                                                      OK (mk_expty arrty, us'')
+                              do szty' <- lift (Types.actual_ty (te ce) (ty szty));
+                              do initty' <- lift (Types.actual_ty (te ce) (ty initty));
+                              check Types.ty_compat szty' Types.INT;
+                              match arrty' with
+                              | Types.ARRAY elty _ => do elty' <- lift (Types.actual_ty (te ce) elty);
+                                                      check Types.ty_compat initty' elty';
+                                                      OK (mk_expty arrty', us'')
                               | _ => ERR
                               end
     end
@@ -290,23 +327,26 @@ Section TYPE_CHECK.
     match var with
     | SimpleVar name => do entry <- lift (Symbol.look (ve ce) name);
                         match entry with
-                        | Env.VarEntry ty => do ty' <- lift (Types.actual_ty ty);
+                        | Env.VarEntry ty => do ty' <- lift (Types.actual_ty (te ce) ty);
                                              OK (mk_expty ty', us)
                         | _ => ERR
                         end
     | FieldVar v field => do (vty, us') <- transVar ce us v;
-                          match ty vty with
+                          do vty' <- lift (Types.actual_ty (te ce) (ty vty));
+                          match vty' with
                           | Types.RECORD ftys _ =>
                               do field' <- lift (rf_find field ftys);
-                              do fieldty <- lift (Types.actual_ty (Types.rf_type field'));
+                              do fieldty <- lift (Types.actual_ty (te ce) (Types.rf_type field'));
                               OK (mk_expty fieldty, us')
                           | _ => ERR
                           end
     | SubscriptVar v idx => do (idxty, us') <- transExp ce us idx;
                             do (vty, us'') <- transVar ce us' v;
-                            check Types.ty_compat (ty idxty) Types.INT;
-                            match ty vty with
-                            | Types.ARRAY elty _ => do elty' <- lift (Types.actual_ty elty);
+                            do idxty' <- lift (Types.actual_ty (te ce) (ty idxty));
+                            do vty' <- lift (Types.actual_ty (te ce) (ty vty));
+                            check Types.ty_compat idxty' Types.INT;
+                            match vty' with
+                            | Types.ARRAY elty _ => do elty' <- lift (Types.actual_ty (te ce) elty);
                                                     OK (mk_expty elty', us'')
                             | _ => ERR
                             end
@@ -315,18 +355,22 @@ Section TYPE_CHECK.
     match dec with
     | FunctionDec decs => OK (ce, us) (* tmp *)
     | VarDec v None val => do (valty, us') <- transExp ce us val;
-                           match ty valty with
+                           do valty' <- lift (Types.actual_ty (te ce) (ty valty));
+                           match valty' with
                            | Types.NIL => ERR
                            | _ => let ve' := Symbol.enter (ve ce) (vd_name v) (Env.VarEntry (ty valty)) in
                                   OK (update_ve ce ve', us')
                            end
     | VarDec v (Some tyname) val => do (valty, us') <- transExp ce us val;
                                     do vty <- lift (Symbol.look (te ce) tyname);
-                                    do vty' <- lift (Types.actual_ty vty);
-                                    check Types.ty_compat (ty valty) vty';
-                                    let ve' := Symbol.enter (ve ce) (vd_name v) (Env.VarEntry (ty valty)) in
+                                    do vty' <- lift (Types.actual_ty (te ce) vty);
+                                    do valty' <- lift (Types.actual_ty (te ce) (ty valty));
+                                    check Types.ty_compat valty' vty';
+                                    let ve' := Symbol.enter (ve ce) (vd_name v) (Env.VarEntry vty) in
                                     OK (update_ve ce ve', us')
-    | TypeDec decs => OK (ce, us) (* tmp *)
+    | TypeDec decs => do te' <- transTydecHeads (te ce) decs;
+                      do (te'', us') <- transTydecs te' us decs;
+                      OK (update_te ce te'', us')
     end
   with transDeclist (ce : composite_env) (us : Types.upool) (decs : declist) : @res (composite_env * Types.upool) :=
     match decs with
@@ -355,12 +399,12 @@ Section TYPE_SPEC.
         wt_op Types.STRING Types.STRING Eq Types.INT
     | wt_eq_arr : forall aty u,
         wt_op (Types.ARRAY aty u) (Types.ARRAY aty u) Eq Types.INT
-    | wt_eq_rec : forall rty u,
-        wt_op (Types.RECORD rty u) (Types.RECORD rty u) Eq Types.INT
-    | wt_eq_lnil : forall rty u,
-        wt_op Types.NIL (Types.RECORD rty u) Eq Types.INT
-    | wt_eq_rnil : forall rty u,
-        wt_op (Types.RECORD rty u) Types.NIL Eq Types.INT.
+    | wt_eq_rec : forall rfs1 rfs2 u,
+        wt_op (Types.RECORD rfs1 u) (Types.RECORD rfs2 u) Eq Types.INT
+    | wt_eq_lnil : forall rfs u,
+        wt_op Types.NIL (Types.RECORD rfs u) Eq Types.INT
+    | wt_eq_rnil : forall rfs u,
+        wt_op (Types.RECORD rfs u) Types.NIL Eq Types.INT.
 
   Inductive wt_fields (te : tenv) (us : Types.upool) : list Symbol.t -> list Types.ty -> Prop :=
     | wt_fnil :
@@ -384,6 +428,24 @@ Section TYPE_SPEC.
         (us', u) = Types.unew us ->
         wt_ty te us (ArrayTy n) (Types.ARRAY ty u) us'.
 
+  Inductive wt_tydec_heads (te : tenv) : list Absyn.tydec -> tenv -> Prop :=
+    | wt_tdh_nil :
+        wt_tydec_heads te nil te
+    | wt_tdh_cons : forall td tds te' te'',
+        Symbol.enter te (td_name td) (Types.NAME (td_name td)) = te' ->
+        wt_tydec_heads te' tds te'' ->
+        wt_tydec_heads te (td :: tds) te''.
+
+  Inductive wt_tydecs (te : tenv) (us : Types.upool) : list Absyn.tydec -> tenv -> Types.upool -> Prop :=
+    | wt_td_nil :
+        wt_tydecs te us nil te us
+    | wt_td_cons : forall td tds ty te' us' te'' us'',
+        wt_ty te us (td_ty td) ty us' ->
+        Symbol.enter te (td_name td) ty = te' ->
+        wt_tydecs te' us' tds te'' us'' ->
+        wt_tydecs te us (td :: tds) te'' us''.
+
+  (* Some of the actual_ty calls may be redundant, but to be safe there should be one before any ty_compat *)
   Inductive wt_exp (ce : composite_env) (us : Types.upool) : Absyn.exp -> Types.ty -> Types.upool -> Prop :=
     | wt_varexp : forall v ty us',
         wt_var ce us v ty us' ->
@@ -394,53 +456,71 @@ Section TYPE_SPEC.
         wt_exp ce us (IntExp n) Types.INT us
     | wt_strexp : forall s,
         wt_exp ce us (StringExp s) Types.STRING us
-    | wt_appexp : forall f args argtys formtys retty us',
+    | wt_appexp : forall f args argtys formtys argtys' formtys' retty us',
         Symbol.look (ve ce) f = Some (Env.FunEntry formtys retty) ->
         wt_explist ce us args argtys us' ->
-        tys_compat argtys formtys = true ->
+        Types.actual_tys (te ce) formtys = Some formtys' ->
+        Types.actual_tys (te ce) argtys = Some argtys' ->
+        tys_compat argtys' formtys' = true ->
         wt_exp ce us (AppExp f args) retty us'
-    | wt_oppexp : forall f l r fty lty rty us' us'',
+    | wt_oppexp : forall f l r fty lty rty lty' rty' us' us'',
         wt_exp ce us l lty us' ->
         wt_exp ce us' r rty us'' ->
-        wt_op lty rty (getOpType f) fty ->
+        Types.actual_ty (te ce) lty = Some lty' ->
+        Types.actual_ty (te ce) rty = Some rty' ->
+        wt_op lty' rty' (getOpType f) fty ->
         wt_exp ce us (OpExp l f r) fty us''
-    | wt_recexp : forall fvals fnames ftys rty ty u fields us',
+    | wt_recexp : forall fvals fnames ftys ftys' rty ty u fields fieldtys us',
         Symbol.look (te ce) rty = Some ty ->
-        Types.actual_ty ty = Some (Types.RECORD fields u) ->
+        Types.actual_ty (te ce) ty = Some (Types.RECORD fields u) ->
         syms_eq fnames (map Types.rf_name fields) = true ->
         wt_explist ce us fvals ftys us' ->
-        tys_compat ftys (map Types.rf_type fields) = true ->
+        Types.actual_tys (te ce) (map Types.rf_type fields) = Some fieldtys ->
+        Types.actual_tys (te ce) ftys = Some ftys' ->
+        tys_compat ftys' fieldtys = true ->
         wt_exp ce us (RecordExp fvals fnames rty) (Types.RECORD fields u) us'
     | wt_seqexp : forall es tys ty us',
         wt_explist ce us es tys us' ->
         ty = last tys Types.UNIT ->
         wt_exp ce us (SeqExp es) ty us'
-    | wt_assignexp : forall v e vty ety us' us'',
+    | wt_assignexp : forall v e vty ety vty' ety' us' us'',
         wt_var ce us v vty us' ->
         wt_exp ce us' e ety us'' ->
-        Types.ty_compat vty ety = true ->
+        Types.actual_ty (te ce) vty = Some vty' ->
+        Types.actual_ty (te ce) ety = Some ety' ->
+        Types.ty_compat vty' ety' = true ->
         Symbol.look (ro ce) (getVarName v) = None ->
         wt_exp ce us (AssignExp v e) Types.UNIT us''
-    | wt_ifthenelseexp : forall p t e tty ety us' us'' us''',
-        wt_exp ce us p Types.INT us' ->
+    | wt_ifthenelseexp : forall p t e pty tty ety tty' ety' us' us'' us''',
+        wt_exp ce us p pty us' ->
         wt_exp ce us' t tty us'' ->
         wt_exp ce us'' e ety us''' ->
-        Types.ty_compat tty ety = true ->
+        Types.actual_ty (te ce) pty = Some Types.INT ->
+        Types.actual_ty (te ce) tty = Some tty' ->
+        Types.actual_ty (te ce) ety = Some ety' ->
+        Types.ty_compat tty' ety' = true -> (* should return whichever of tty and ety is not nil if possible *)
         wt_exp ce us (IfExp p t (Some e)) tty us'''
-    | wt_ifthenexp : forall p t us' us'',
-        wt_exp ce us p Types.INT us' ->
-        wt_exp ce us' t Types.UNIT us'' ->
+    | wt_ifthenexp : forall p t pty tty us' us'',
+        wt_exp ce us p pty us' ->
+        wt_exp ce us' t tty us'' ->
+        Types.actual_ty (te ce) pty = Some Types.INT ->
+        Types.actual_ty (te ce) tty = Some Types.UNIT ->
         wt_exp ce us (IfExp p t None) Types.UNIT us''
-    | wt_whileexp : forall g b us' us'',
-        wt_exp ce us g Types.INT us' ->
-        wt_exp (incr_ll ce) us' b Types.UNIT us'' ->
+    | wt_whileexp : forall g b gty bty us' us'',
+        wt_exp ce us g gty us' ->
+        wt_exp (incr_ll ce) us' b bty us'' ->
+        Types.actual_ty (te ce) gty = Some Types.INT ->
+        Types.actual_ty (te ce) bty = Some Types.UNIT ->
         wt_exp ce us (WhileExp g b) Types.UNIT us''
-    | wt_forexp : forall v lo hi b us' us'' us''' ve' ro',
-        wt_exp ce us lo Types.INT us' ->
-        wt_exp ce us' hi Types.INT us'' ->
+    | wt_forexp : forall v lo hi loty hity b bty us' us'' us''' ve' ro',
+        wt_exp ce us lo loty us' ->
+        wt_exp ce us' hi hity us'' ->
+        Types.actual_ty (te ce) loty = Some Types.INT ->
+        Types.actual_ty (te ce) hity = Some Types.INT ->
         Symbol.enter (ve ce) (vd_name v) (Env.VarEntry Types.INT) = ve' ->
         Symbol.enter (ro ce) (vd_name v) tt = ro' ->
-        wt_exp (incr_ll (update_ve (update_ro ce ro') ve')) us'' b Types.UNIT us''' ->
+        wt_exp (incr_ll (update_ve (update_ro ce ro') ve')) us'' b bty us''' ->
+        Types.actual_ty (te ce) bty = Some Types.UNIT ->
         wt_exp ce us (ForExp v lo hi b) Types.UNIT us'''
     | wt_breakexp :
         0 < ll ce ->
@@ -449,12 +529,15 @@ Section TYPE_SPEC.
         wt_declist ce us decs ce' us' ->
         wt_exp ce' us' e ty us'' ->
         wt_exp ce us (LetExp decs e) ty us''
-    | wt_arrexp : forall aty ty ty' sz init initty u us' us'',
+    | wt_arrexp : forall aty ty ty' ty'' sz szty init initty initty' u us' us'',
         Symbol.look (te ce) aty = Some ty ->
-        Types.actual_ty ty = Some (Types.ARRAY ty' u) ->
-        wt_exp ce us sz Types.INT us' ->
+        Types.actual_ty (te ce) ty = Some (Types.ARRAY ty' u) ->
+        wt_exp ce us sz szty us' ->
         wt_exp ce us' init initty us'' ->
-        Types.ty_compat ty' initty = true ->
+        Types.actual_ty (te ce) szty = Some Types.INT ->
+        Types.actual_ty (te ce) ty' = Some ty'' ->
+        Types.actual_ty (te ce) initty = Some initty' ->
+        Types.ty_compat ty'' initty' = true ->
         wt_exp ce us (ArrayExp aty sz init) (Types.ARRAY ty' u) us''
   with wt_explist (ce : composite_env) (us : Types.upool) : Absyn.explist -> list Types.ty -> Types.upool -> Prop :=
     | wt_enil :
@@ -466,35 +549,43 @@ Section TYPE_SPEC.
   with wt_var (ce : composite_env) (us : Types.upool) : Absyn.var -> Types.ty -> Types.upool -> Prop :=
     | wt_svar : forall n ty ty',
         Symbol.look (ve ce) n = Some (Env.VarEntry ty) ->
-        Types.actual_ty ty = Some ty' ->
+        Types.actual_ty (te ce) ty = Some ty' ->
         wt_var ce us (SimpleVar n) ty' us
-    | wt_fvar : forall v f fs u ty ty' us',
-        wt_var ce us v (Types.RECORD fs u) us' ->
+    | wt_fvar : forall v vty f fs u ty ty' us',
+        wt_var ce us v vty us' ->
+        Types.actual_ty (te ce) vty = Some (Types.RECORD fs u) ->
         rf_in (Types.mk_rfield f ty) fs = true ->
-        Types.actual_ty ty = Some ty' ->
+        Types.actual_ty (te ce) ty = Some ty' ->
         wt_var ce us (FieldVar v f) ty' us'
-    | wt_ssvar : forall v idx u ty ty' us' us'',
-        wt_exp ce us idx Types.INT us' ->
-        wt_var ce us' v (Types.ARRAY ty u) us'' ->
-        Types.actual_ty ty = Some ty' ->
+    | wt_ssvar : forall v idx u idxty vty ty ty' us' us'',
+        wt_exp ce us idx idxty us' ->
+        wt_var ce us' v vty us'' ->
+        Types.actual_ty (te ce) idxty = Some Types.INT ->
+        Types.actual_ty (te ce) vty = Some (Types.ARRAY ty u) ->
+        Types.actual_ty (te ce) ty = Some ty' ->
         wt_var ce us (SubscriptVar v idx) ty' us''
   with wt_dec (ce : composite_env) (us : Types.upool) : Absyn.dec -> composite_env -> Types.upool -> Prop :=
     | wt_fundec : forall fs, (* tmp *)
         wt_dec ce us (FunctionDec fs) ce us
-    | wt_vardec_noty : forall v e ety ve' us',
+    | wt_vardec_noty : forall v e ety ety' ve' us',
         wt_exp ce us e ety us' ->
-        ety <> Types.NIL ->
+        Types.actual_ty (te ce) ety = Some ety' ->
+        ety' <> Types.NIL ->
         Symbol.enter (ve ce) (vd_name v) (Env.VarEntry ety) = ve' ->
         wt_dec ce us (VarDec v None e) (update_ve ce ve') us'
-    | wt_vardec_ty : forall v e tyname ty ty' ety ve' us',
+    | wt_vardec_ty : forall v e tyname ty ty' ety ety' ve' us',
         Symbol.look (te ce) tyname = Some ty ->
-        Types.actual_ty ty = Some ty' ->
         wt_exp ce us e ety us' ->
-        Types.ty_compat ety ty' = true ->
-        Symbol.enter (ve ce) (vd_name v) (Env.VarEntry ety) = ve' ->
+        Types.actual_ty (te ce) ty = Some ty' ->
+        Types.actual_ty (te ce) ety = Some ety' ->
+        Types.ty_compat ety' ty' = true ->
+        Symbol.enter (ve ce) (vd_name v) (Env.VarEntry ty) = ve' ->
         wt_dec ce us (VarDec v (Some tyname) e) (update_ve ce ve') us'
-    | wt_tydec : forall tys us', (* tmp *)
-        wt_dec ce us (TypeDec tys) ce us'
+    | wt_tydec : forall tds te' te'' us',
+        wt_tydec_heads (te ce) tds te' ->
+        wt_tydecs te' us tds te'' us' ->
+        (* check for cycles *)
+        wt_dec ce us (TypeDec tds) (update_te ce te'') us'
   with wt_declist (ce : composite_env) (us : Types.upool) : declist -> composite_env -> Types.upool -> Prop :=
     | wt_dnil :
         wt_declist ce us DNil ce us
@@ -508,31 +599,74 @@ Section TYPE_SPEC.
         wt_exp base_cenv Types.uinit p ty us' ->
         wt_prog p ty us'.
 
+End TYPE_SPEC.
+
+Section SOUNDNESS.
+
+  Ltac type_subst := match goal with
+                     | [ H1 : lift (Types.actual_ty _ ?X) = OK ?Y,
+                         H2 : Types.ty_compat ?Y ?Z = true
+                         |- Types.actual_ty _ ?X = Some ?Z ] =>
+                       solve [apply Types.ty_compat_simpl_eq in H2; apply lift_option in H1; subst; auto]
+                     end.
+
+  Ltac sound_solve H := monadInv H; econstructor; eauto; try type_subst.
+
+  Local Hint Resolve lift_option.
+  Local Hint Resolve Types.ty_compat_sym.
+
+  (* This depends on some details of ty_compat and others that it shouldn't *)
   Lemma transOp_sound : forall l r f ety,
     transOp l r f = OK ety ->
-    wt_op (ty l) (ty r) f (ty ety).
+    wt_op l r f (ty ety).
   Proof.
     destruct f; intros; unfold transOp in H; simpl in H;
-    destruct (Types.ty_compat (ty l) (ty r)) eqn:?; try discriminate;
-    destruct (ty l); inversion H;
-    destruct (ty r); try discriminate;
+    destruct (Types.ty_compat l r) eqn:?; try discriminate;
+    destruct l; inversion H;
+    destruct r; try discriminate;
     try constructor;
-    unfold Types.ty_compat in Heqb; destruct Types.ty_dec; try discriminate; inversion e; constructor.
+    try (unfold Types.ty_compat in Heqb; destruct Types.ty_dec; try discriminate; inversion e; constructor).
+    unfold Types.ty_compat in Heqb; destruct Types.ty_dec; try discriminate. inversion e. constructor.
+    destruct (Unique.unique_dec t t0); try discriminate. subst. constructor.
   Qed.
+
+  Local Hint Resolve transOp_sound.
 
   Lemma transFields_sound : forall te us fs tys,
     transFields te us fs = OK tys ->
     wt_fields te us fs tys.
   Proof.
-    induction fs; intros; monadInv H; constructor; auto using lift_option.
+    induction fs; intros; sound_solve H.
   Qed.
+
+  Local Hint Resolve transFields_sound.
 
   Lemma transTy_sound : forall te us abty ty us',
     transTy te us abty = OK (ty, us') ->
     wt_ty te us abty ty us'.
   Proof.
-    destruct abty; intros; monadInv H; constructor; auto using lift_option, transFields_sound.
+    destruct abty; intros; sound_solve H.
   Qed.
+
+  Local Hint Resolve transTy_sound.
+
+  Lemma transTydecHeads_sound : forall te tds te',
+    transTydecHeads te tds = OK te' ->
+    wt_tydec_heads te tds te'.
+  Proof.
+    intros; generalize dependent te0; induction tds; intros; [sound_solve H | econstructor; eauto].
+  Qed.
+
+  Local Hint Resolve transTydecHeads_sound.
+
+  Lemma transTydecs_sound : forall te us tds te' us',
+    transTydecs te us tds = OK (te', us') ->
+    wt_tydecs te us tds te' us'.
+  Proof.
+    intros; generalize dependent te0; generalize dependent us; induction tds; intros; sound_solve H.
+  Qed.
+
+  Local Hint Resolve transTydecs_sound.
 
   Theorem transExp_sound : forall ce us e ety us',
     transExp ce us e = OK (ety, us') ->
@@ -550,8 +684,7 @@ Section TYPE_SPEC.
     transDeclist ce us ds = OK (ce', us') ->
     wt_declist ce us ds ce' us'.
   Proof.
-    - destruct e; intros;
-      try solve [monadInv H; econstructor; eauto using lift_option, transOp_sound].
+    - destruct e; intros; try solve [sound_solve H].
       + simpl in H; constructor; auto.
       + monadInv H; destruct e.
         * monadInv EQ; econstructor; [econstructor | reflexivity].
@@ -563,55 +696,40 @@ Section TYPE_SPEC.
             - intros; simpl; rewrite <- IHxs; destruct xs; reflexivity.
           }
           apply Htymap.
-      + destruct o; monadInv H.
-        * econstructor; eauto.
-          apply transExp_sound in EQ; destruct (ty x); try discriminate; eassumption.
-        * econstructor.
-          apply transExp_sound in EQ; destruct (ty x); try discriminate; eassumption.
-          apply transExp_sound in EQ1; destruct (ty x1); try discriminate; eassumption.
-      + monadInv H; econstructor. (* Should make a tactic or lemma for this pattern *)
-        apply transExp_sound in EQ; destruct (ty x); try discriminate; eassumption.
-        apply transExp_sound in EQ1; destruct (ty x1); try discriminate; eassumption.
-      + monadInv H; econstructor; eauto.
-        apply transExp_sound in EQ; destruct (ty x); try discriminate; eassumption.
-        apply transExp_sound in EQ1; destruct (ty x1); try discriminate; eassumption.
-        apply transExp_sound in EQ4; destruct (ty x3); try discriminate; eassumption.
       + monadInv H; constructor.
         unfold lt; fold (leb 1 (ll ce)) in EQ; auto using leb_complete.
-      + monadInv H; econstructor; eauto using lift_option, Types.ty_compat_sym. (* should make a hint database *)
-        apply transExp_sound in EQ1; destruct (ty x0); try discriminate; eassumption.
-    - destruct es; intros; monadInv H; econstructor; eauto.
-    - destruct v; intros.
-      + monadInv H; econstructor; eauto using lift_option.
-      + monadInv H; econstructor; eauto using lift_option.
-        apply transVar_sound in EQ; rewrite HEQ in EQ; eassumption.
-        { apply lift_option in EQ1.
-          pose proof EQ1.
-          apply rf_find_in in EQ1.
+    - destruct es; intros; sound_solve H.
+    - destruct v; intros;
+      try solve [sound_solve H].
+      + monadInv H; econstructor; eauto.
+        { apply lift_option in EQ0.
+          pose proof EQ0.
+          apply rf_find_in in EQ0.
           apply rf_find_name in H.
-          erewrite rf_eq_in. apply EQ1.
+          erewrite rf_eq_in. eassumption.
           apply sym_eq_rf_eq.
-          fold (Types.rf_name x1).
-          rewrite Symbol.eq_sym; apply H.
+          fold (Types.rf_name x2).
+          rewrite Symbol.eq_sym; assumption.
         }
-      + monadInv H; econstructor; eauto using lift_option.
-        apply transExp_sound in EQ; destruct (ty x); try discriminate; eassumption.
-        apply transVar_sound in EQ1; rewrite HEQ in EQ1; eassumption.
     - destruct d; intros.
       + monadInv H; constructor. (* tmp *)
-      + destruct o.
-        * monadInv H; econstructor; eauto using lift_option.
-        * monadInv H; econstructor; eauto; subst; congruence.
-      + monadInv H; constructor. (* tmp *)
-    - destruct ds; intros; monadInv H; econstructor; eauto.
+      + destruct o; monadInv H; econstructor; eauto; congruence.
+      + sound_solve H.
+    - destruct ds; intros; sound_solve H.
   Qed.
+
+  Local Hint Resolve transExp_sound.
 
   Theorem transProg_sound : forall p ety us',
     transProg p = OK (ety, us') ->
     wt_prog p (ty ety) us'.
   Proof.
-    unfold transProg; constructor; auto using transExp_sound.
+    unfold transProg; constructor; auto.
   Qed.
+
+End SOUNDNESS.
+
+Section COMPLETENESS.
 
   Theorem transExp_complete : forall ce us e ety us',
     wt_exp ce us e (ty ety) us' ->
@@ -638,10 +756,4 @@ Section TYPE_SPEC.
     intros; unfold transProg; inversion H; auto using transExp_complete.
   Qed.
 
-  Lemma transExp_not_name : forall ce us e ety us' n oty,
-    transExp ce us e = OK (ety, us') ->
-    ty ety <> Types.NAME n oty.
-  Proof.
-  Admitted.
-
-End TYPE_SPEC.
+End COMPLETENESS.
